# baseURI: https://www.w3.org/2006/time/agg
# imports: http://purl.org/dc/elements/1.1/
# imports: http://www.w3.org/2006/time

@prefix dct: <http://purl.org/dc/terms/> .
@prefix owl: <http://www.w3.org/2002/07/owl#> .
@prefix rdf: <http://www.w3.org/1999/02/22-rdf-syntax-ns#> .
@prefix rdfs: <http://www.w3.org/2000/01/rdf-schema#> .
@prefix skos: <http://www.w3.org/2004/02/skos/core#> .
@prefix time: <http://www.w3.org/2006/time#> .
@prefix xsd: <http://www.w3.org/2001/XMLSchema#> .

time:TemporalAggregate
  a owl:Class ;
  rdfs:comment """A temporal aggregate is temporal entity that is an aggregation of temporal entities

Note: no ordering relationships are implied amongst the parts. Relationships between temporal entities are supported by explicit properties, such as time:after time:intervalMeets, etc""" ;
  rdfs:label "Temporal aggregate" ;
  rdfs:subClassOf time:TemporalEntity ;
  rdfs:subClassOf [
      a owl:Restriction ;
      owl:minCardinality "1"^^xsd:nonNegativeInteger ;
      owl:onProperty time:hasPart ;
    ] ;
  skos:example """
ex:VicSchoolTerms2020
  a time:TemporalAggregate ;
  rdfs:label \"Public school year - Victoria 2020 \" ;
  time:hasBeginning ex:t1b ;
  time:hasEnd ex:t4e ;
  time:hasPart ex:t1 ;
  time:hasPart ex:t2 ;
  time:hasPart ex:t3 ;
  time:hasPart ex:t4 ;
.
""" ;
.
time:hasPart
  a owl:ObjectProperty ;
  rdfs:comment "Link to a temporal entity that is a part of this temporal aggregate" ;
  rdfs:domain time:TemporalAggregate ;
  rdfs:label "has a part" ;
  rdfs:range time:TemporalEntity ;
  rdfs:subPropertyOf dct:hasPart ;
  rdfs:subPropertyOf rdfs:member ;
  skos:example """
ex:VicSchoolTerms2020
  a time:TemporalAggregate ;
  time:hasPart ex:t1 ;
.
ex:t1
  a time:ProperInterval ;
.
""" ;
.
time:isPartOf
  a owl:ObjectProperty ;
  rdfs:comment "Link to a temporal aggregate of which this temporal entity is a part" ;
  rdfs:domain time:TemporalEntity ;
  rdfs:label "is a part of" ;
  rdfs:range time:TemporalAggregate ;
  owl:inverseOf time:hasPart ;
  skos:example """
ex:t1
  a time:ProperInterval ;
  time:isPartOf ex:VicSchoolTerms2020 ;
.
ex:VicSchoolTerms2020
  a time:TemporalAggregate ;
.
""" ;
.
<https://www.w3.org/2006/time/agg>
  a owl:Ontology ;
  dct:created "2020-01-16"^^xsd:date ;
  dct:creator <https://orcid.org/0000-0002-3884-3420> ;
  dct:license <https://creativecommons.org/share-your-work/public-domain/cc0/> ;
  dct:modified "2020-04-17"^^xsd:date ;
  dct:title "An extension of OWL-Time for temporal aggregates" ;
  rdfs:label "Temporal aggregates" ;
  rdfs:comment """This document describes some extensions to OWL-Time to represent temporal entities composed of other temporal entities. 
  New classes and properties are specified in the original OWL-Time namespace. 
  The classes, properties, and axioms in this RDF graph are described in https://w3c.github.io/sdw/time-aggregates/
  Their status is non-normative, and OWL-Time applications are not required to recognize or support them. """ ;
  owl:imports <http://purl.org/dc/elements/1.1/> ;
  owl:imports <http://www.w3.org/2006/time> ;
.
